src/high/viewobjective.v
@@ -1,0 +1,163 @@
+From iris.bi Require Export monpred.
+From iris.proofmode Require Import monpred tactics.
+From iris.base_logic.lib Require Import iprop.
+
+From self.high Require Import dprop dprop_liftings.
+
+Program Definition monPred_view_objectively_def {Σ} (P : dProp Σ) : dProp Σ :=
+  MonPred (λ i, ∀ TV, P (TV, i.2))%I _.
+Next Obligation.
+  intros.
+  intros [? gnames].
+  introsIndex ? ?.
+  naive_solver.
+Qed.
+Definition monPred_view_objectively_aux : seal (@monPred_view_objectively_def).
+Proof. by eexists. Qed.
+Definition monPred_view_objectively :=
+  monPred_view_objectively_aux.(unseal).
+Definition monPred_view_objectively_eq : @monPred_view_objectively = _ :=
+  monPred_view_objectively_aux.(seal_eq).
+
+Global Arguments monPred_view_objectively {_} _%I.
+
+Notation "'<vobj>' P" := (monPred_view_objectively P) (at level 20, right associativity) : bi_scope.
+
+(* Expresses that a proposition holds independently of the thread view but may
+   still depend on the ghost names. *)
+Class ViewObjective {Σ} (P : dProp Σ) :=
+  view_objective_at TV1 TV2 gnames : P (TV1, gnames) -∗ P (TV2, gnames).
+Global Arguments ViewObjective {_} _%I.
+Global Arguments view_objective_at {_} _%I {_}.
+Global Hint Mode ViewObjective + ! : typeclass_instances.
+Global Instance: Params (@Objective) 1 := {}.
+
+Section view_objective_instances.
+  Context {Σ : gFunctors}.
+
+  Implicit Types (P : dProp Σ).
+  Implicit Types (Pi : iProp Σ).
+
+  Lemma monPred_objectively_unfold :
+    monPred_view_objectively = λ P, lift_d (λ nD, ∀ TV, P (TV, nD))%I.
+  Proof.
+    rewrite monPred_view_objectively_eq.
+    rewrite /monPred_view_objectively_def.
+    simpl.
+  Admitted.
+
+  Lemma view_objective_objective P : Objective P → ViewObjective P.
+  Proof.
+    rewrite /Objective.
+    rewrite /ViewObjective.
+    naive_solver.
+  Qed.
+
+  Global Instance embed_objective (P : iProp Σ) : ViewObjective (⎡ P ⎤ : dProp Σ)%I.
+  Proof.
+    rewrite /ViewObjective.
+    setoid_rewrite monPred_at_embed.
+    naive_solver.
+  Qed.
+
+  Global Instance with_gnames_view_objective (P : nvmDeltaG → dProp Σ) :
+    (∀ gnames, ViewObjective (P gnames)) → ViewObjective (with_gnames P).
+  Proof.
+    rewrite /ViewObjective.
+    intros Ho.
+    iIntros.
+    iApply Ho.
+    iFrame.
+  Qed.
+
+  Lemma monPred_at_view_objectively i P : (<vobj> P) i ⊣⊢ ∀ TV, P (TV, i.2).
+  Proof. by rewrite monPred_view_objectively_eq. Qed.
+
+  Lemma view_objective_view_objectively P `{!ViewObjective P} : P ⊢ <vobj> P.
+  Proof.
+    iModel.
+    rewrite monPred_at_view_objectively.
+    simpl.
+    iIntros "H" (?).
+    iApply view_objective_at.
+    done.
+  Qed.
+
+  Global Instance embed_view_objective Pi : ViewObjective ⎡ Pi ⎤.
+  Proof. apply view_objective_objective. apply _. Qed.
+  Global Instance pure_view_objective φ : ViewObjective (⌜ φ ⌝ : dProp Σ)%I.
+  Proof. apply view_objective_objective. apply _. Qed.
+  Global Instance emp_view_objective : ViewObjective (emp : dProp Σ)%I.
+  Proof. apply view_objective_objective. apply _. Qed.
+  Global Instance objectively_view_objective P : ViewObjective (<vobj> P).
+  Proof. rewrite monPred_view_objectively_eq. done. Qed.
+
+  Global Instance and_view_objective P Q `{!ViewObjective P, !ViewObjective Q} : ViewObjective (P ∧ Q).
+  Proof.
+    iIntros (i j ?).
+    rewrite 2!monPred_at_and. rewrite 2!(view_objective_at _ i j).
+    done.
+  Qed.
+  Global Instance or_view_objective P Q `{!ViewObjective P, !ViewObjective Q} : ViewObjective (P ∨ Q).
+  Proof.
+    intros i j ?. rewrite 2!monPred_at_or. rewrite 2!(view_objective_at _ i j). done.
+  Qed.
+  (* Global Instance impl_view_objective P Q `{!ViewObjective P, !ViewObjective Q} : ViewObjective (P → Q). *)
+  (* Proof. *)
+  (*   intros i j. unseal. rewrite (bi.forall_elim i) bi.pure_impl_forall. *)
+  (*   rewrite bi.forall_elim //. apply bi.forall_intro=> k. *)
+  (*   rewrite bi.pure_impl_forall. apply bi.forall_intro=>_. *)
+  (*   rewrite (objective_at Q i). by rewrite (objective_at P k). *)
+  (* Qed. *)
+  Global Instance forall_view_view_objective (A : Type) (Φ : A → dProp Σ) :
+    (∀ x : A, ViewObjective (Φ x)) → ViewObjective (∀ x : A, Φ x).
+  Proof.
+    iIntros (????).
+    rewrite 2!monPred_at_forall.
+    iIntros "?" (?).
+    iApply view_objective_at.
+    iAssumption.
+  Qed.
+  (* Global Instance exists_view_objective {A} Φ {H : ∀ x : A, ViewObjective (Φ x)} : *)
+  (*   @ViewObjective I PROP (∃ x, Φ x)%I. *)
+  (* Proof. intros i j. unseal. do 2 f_equiv. by apply objective_at. Qed. *)
+
+  (* Global Instance sep_view_objective P Q `{!ViewObjective P, !ViewObjective Q} : ViewObjective (P ∗ Q). *)
+  (* Proof. intros i j. unseal. by rewrite !(objective_at _ i j). Qed. *)
+  Global Instance sep_view_objective P Q :
+    ViewObjective P → ViewObjective Q → ViewObjective (P ∗ Q).
+  Proof.
+    intros ? ? i j ?.
+    rewrite 2!monPred_at_sep. rewrite 2!(view_objective_at _ i j).
+    done.
+  Qed.
+
+  Global Instance wand_view_objective P Q `{!ViewObjective P, !ViewObjective Q} : ViewObjective (P -∗ Q).
+  Proof.
+    iIntros (i j ?) "w".
+    introsIndex ? ?.
+    rewrite (view_objective_at _ p i).
+    iIntros "P".
+    iSpecialize ("w" with "P").
+    rewrite (view_objective_at Q i p).
+    done.
+  Qed.
+  (* Global Instance persistently_view_objective P `{!ViewObjective P} : ViewObjective (<pers> P). *)
+  (* Proof. intros i j. unseal. by rewrite objective_at. Qed. *)
+
+  (* Global Instance affinely_view_objective P `{!ViewObjective P} : ViewObjective (<affine> P). *)
+  (* Proof. rewrite /bi_affinely. apply _. Qed. *)
+  (* Global Instance intuitionistically_view_objective P `{!ViewObjective P} : ViewObjective (□ P). *)
+  (* Proof. rewrite /bi_intuitionistically. apply _. Qed. *)
+  (* Global Instance absorbingly_view_objective P `{!ViewObjective P} : ViewObjective (<absorb> P). *)
+  (* Proof. rewrite /bi_absorbingly. apply _. Qed. *)
+  (* Global Instance persistently_if_view_objective P p `{!ViewObjective P} : ViewObjective (<pers>?p P). *)
+  (* Proof. rewrite /bi_persistently_if. destruct p; apply _. Qed. *)
+  (* Global Instance affinely_if_view_objective P p `{!ViewObjective P} : ViewObjective (<affine>?p P). *)
+  (* Proof. rewrite /bi_affinely_if. destruct p; apply _. Qed. *)
+  (* Global Instance absorbingly_if_view_objective P p `{!ViewObjective P} : ViewObjective (<absorb>?p P). *)
+  (* Proof. rewrite /bi_absorbingly_if. destruct p; apply _. Qed. *)
+  (* Global Instance intuitionistically_if_view_objective P p `{!ViewObjective P} : ViewObjective (□?p P). *)
+  (* Proof. rewrite /bi_intuitionistically_if. destruct p; apply _. Qed. *)
+
+End view_objective_instances.
